Nominal instances and fresh update

theories/Fresh.v
@@ -1,26 +1,19 @@
 From Nominal Require Import Nominal.
 
-(* Freshness *)
-Definition fresh_e `{Nominal X} (a: name) (x: X) :=
-  ∃ (b : name), b ∉ support x ∧ ⟨a,b⟩ • x ≡@{X} x.
+Record freshT `{Nominal X} (a : name) (x : X) : Type := mkFreshT {
+  new : name;
+  new_fresh : new ∉ support x;
+  new_fixpoint : ⟨a,new⟩ • x ≡@{X} x
+}.
 
-Definition fresh_a `{Nominal X} (a: name) (x: X) :=
-  ∀ (b : name), b ∉ support x → ⟨a,b⟩ • x ≡ x.
+Definition freshP_e `{Nominal X} (a: name) (x: X) := ∃ (b : name), b ∉ support x ∧ ⟨a,b⟩ • x ≡@{X} x.
+Definition freshP_a `{Nominal X} (a: name) (x: X) := ∀ (b : name), b ∉ support x → ⟨a,b⟩ • x ≡@{X} x.
 
-(* Infix "#" := freshness (at level 50). *)
-Infix "#ₑ" := fresh_e (at level 50).
-Infix "#ₐ" := fresh_a (at level 50).
+Infix "#" := freshT (at level 50).
+Infix "#ₚₑ" := freshP_e (at level 50).
+Infix "#ₚₐ" := freshP_a (at level 50).
 
-(* Lemma some_any `{Nominal X} (a b : name) (x : X) : 
-  b ∉ support x → ⟨a,b⟩ • x ≡@{X} x → (∀ c, c ∉ support x → ⟨a,c⟩ • x ≡@{X} x).
-Proof.
-  intros; destruct (decide (c = a)), (decide (c = b)); subst; auto.
-  - apply perm_action_equal.
-  - rewrite perm_expand with (b := b); 
-      try rewrite <-2!gact_compat, H2, (support_spec _ b c); auto.
-Qed. *)
-
-Lemma some_any `{Nominal X} (a: name) (x: X) : a #ₑ x ↔ a #ₐ x.
+Lemma some_any `{Nominal X} (a: name) (x: X) : a #ₚₑ x ↔ a #ₚₐ x.
 Proof.
   split.
   - intros [b [SB HH]] c SC; destruct (decide (c = a)), (decide (c = b)); subst; auto.
@@ -31,16 +24,46 @@ Proof.
     + apply HH, is_fresh.
 Qed.
 
-Lemma support_fresh_e `{Nominal X} (a : name) (x: X):
-  a ∉ support x → a #ₑ x.
+Lemma fresh_spec_el `{Nominal X} (a: name) (x: X) : a # x → a #ₚₑ x.
+Proof. intros [n ? ?]; exists n; split; auto. Qed.
+
+Lemma fresh_spec_al `{Nominal X} (a: name) (x: X) : a # x → a #ₚₐ x.
+Proof. intro; apply some_any, fresh_spec_el; auto. Qed.
+
+Definition fresh_spec_ar `{Nominal X} (a: name) (x: X) : a #ₚₐ x → a # x.
+Proof. 
+  intros HH; constructor 1 with (fresh (support x)); pose proof (is_fresh (support x));
+    specialize (HH (fresh (support x)) H1); auto.
+Defined.
+
+Definition fresh_spec_er `{Nominal X} (a: name) (x: X) : a #ₚₑ x → a # x.
+Proof. intros HH; apply fresh_spec_ar, some_any; assumption. Defined.
+
+Lemma support_fresh `{Nominal X} (a : name) (x: X): a ∉ support x → a # x.
+Proof. intros; econstructor; [idtac | eapply perm_action_equal]; auto. Qed.
+
+Definition update_fresh `{Nominal X} (a b: name) (x: X) : a # x → b ∉ support x → a # x.
+Proof. intros F ?; eapply fresh_spec_al in F; unfold freshP_a in F; econstructor; eauto. Defined. 
+
+(* Lemma support_fresh_a `{Nominal X} (a : name) (x: X): a ∉ support x → a #ₐ x.
+Proof. intros; apply some_any, support_fresh_e; auto. Qed. *)
+
+Lemma fresh_support_fresh `{Nominal X} (x: X): fresh (support x) # x.
+Proof. constructor 1 with (fresh (support x)); [apply is_fresh | apply perm_action_equal]. Qed.
+
+Lemma fresh_fixpoint `{Nominal X} (a b : name) (x : X) : a # x → b # x → ⟨a,b⟩ • x ≡ x.
 Proof.
-  intros; exists a; split; [idtac | apply perm_action_equal]; auto.
-Qed.
-
-Lemma support_fresh_a `{Nominal X} (a : name) (x: X): a ∉ support x → a #ₐ x.
-Proof. intros; apply some_any, support_fresh_e; auto. Qed.
-
-Lemma fresh_support_fresh `{Nominal X} (x: X): fresh (support x) #ₑ x.
-Proof. unfold fresh_e; exists (fresh (support x)); split;
-        [apply is_fresh | apply perm_action_equal].
+  intros FA FB; destruct (decide (a = b)); subst.
+  - apply perm_action_equal.
+  - destruct FA as [p ? Fp]; destruct FB as [k ? Fk]; 
+      destruct (decide (p = k)), (decide (k = a)), (decide (k = b)), 
+        (decide (p = a)), (decide (p = b)); subst;
+          try first [assumption | apply perm_action_equal | rewrite perm_swap; assumption]. 
+    + rewrite (perm_expand _ k _), <-!gact_compat, Fp, (perm_swap k b), Fk; auto; apply Fp.
+    + apply support_spec; auto. 
+    + rewrite (perm_expand _ p _), <-!gact_compat, Fp, (support_spec _ p b); auto.
+    + rewrite (perm_expand _ k _), <-!gact_compat, (support_spec x a k), (perm_swap k b), 
+        Fk, support_spec; auto. 
+    + rewrite (perm_expand _ p _), (perm_expand p k b), !grp_assoc, <-!gact_compat, 
+        Fp, (perm_swap k b), (support_spec x p k), Fk, (support_spec x p k), Fp; auto.
 Qed.
