theories/Instances/Name.v
@@ -1,0 +1,31 @@
+(* Name forms a nominal set *)
+From Nominal Require Import Atom Nominal Fresh.
+
+Instance name_action : PermAct name := swap_perm.
+Instance name_equiv : Equiv name := eq.
+Instance name_support : Support name := singleton.
+
+Instance name_perm : Perm name.
+Proof. 
+    split; unfold "≡",name_equiv,action, prmact, name_action in *; repeat intro.
+    - typeclasses eauto.
+    - subst; rewrite H; auto.
+    - auto.
+    - symmetry; apply swap_perm_app.
+Defined.
+
+Instance name_nominal : Nominal name.
+Proof. split; intros; [apply name_perm | apply swap_neither1; apply not_elem_of_singleton]; auto. Qed.
+
+Lemma name_fresh_neq (a b : name) : a # b → a ≠ b.
+Proof. 
+    intros [c ? cF]; destruct (decide (a = c)); subst.
+    - apply not_elem_of_singleton; auto.
+    - apply swap_neither2 in cF as [[] | []]; subst; auto.
+Qed.  
+
+Definition name_neq_fresh (a b : name) : a ≠ b → a # b.
+Proof. 
+    intros; constructor 1 with a; 
+        [unfold support; apply not_elem_of_singleton | apply swap_neither1]; auto. 
+Qed. 
